src/Char.v
@@ -1,0 +1,42 @@
+Require Import Category.
+Require Import Induction.
+Require Import Combinators.
+Require Import Sized.
+Require Import NEList.
+
+Require Import Ascii.
+Require Import StringAsList.
+
+Require Import Coq.Lists.List.
+Import ListNotations.
+
+Section Char.
+
+Context {M : Type -> Type} {Chars : nat -> Type} {A : Type} {n : nat}.
+
+Definition char `{RawAlternative M} `{RawMonad M} `{Sized Chars ascii}
+  (c : ascii) : Parser Chars ascii M ascii n := exact c.
+
+Definition space `{RawAlternative M} `{RawMonad M} `{Sized Chars ascii}
+  : Parser Chars ascii M ascii n := anyOf (" " :: "009" :: "013" :: [])%char.
+
+Definition spaces `{RawAlternative M} `{RawMonad M} `{Sized Chars ascii}
+  : Parser Chars ascii M (NEList ascii) n := nelist space.
+
+Definition text `{RawAlternative M} `{RawMonad M} `{Sized Chars ascii}
+  (t : String) `{NonEmpty ascii t} : Parser Chars ascii M String n :=
+  Combinators.map NEList.toList (exacts nonEmpty).
+
+Definition parens `{RawMonad M} `{RawAlternative M} `{Sized Chars ascii}
+  (p : Box (Parser Chars ascii M A) n) : Parser Chars ascii M A n :=
+  between (char "(") (char ")") p.
+
+Definition parensm `{RawMonad M} `{RawAlternative M} `{Sized Chars ascii}
+  (p : Parser Chars ascii M A n) : Parser Chars ascii M A n :=
+  betweenm (char "(") (char ")") p.
+
+Definition withSpaces `{RawMonad M} `{RawAlternative M} `{Sized Chars ascii}
+  (p : Parser Chars ascii M A n) : Parser Chars ascii M A n :=
+  spaces ?&> p <&? spaces.
+
+End Char.
