src/StringAsList.v
@@ -1,0 +1,16 @@
+Require Import Ascii.
+Require Import String.
+
+Require Import Coq.Lists.List.
+Import ListNotations.
+
+Definition String := list ascii.
+
+Fixpoint fromString (s : string) : String :=
+match s with
+ | String.EmptyString => []
+ | String.String c s' => c :: fromString s'
+end.
+
+Fixpoint toString (s : String) : string :=
+  fold_right String.String String.EmptyString s.
